refined the loop invariant + started working on loop verification

specs/verif_hmac_drbg_update.v
@@ -31,19 +31,87 @@ Proof.
   destruct provided_data; reflexivity.
 Qed.
 
-Definition update_loop_invariant ctx sep provided_data old_key old_value state_abs state i key value :=
-  (*
-  EX i: _, EX key: _, EX value: _,
-   *)
-  PROP  ((key, value) = HMAC_DRBG_update_round HMAC256 provided_data old_key old_value 0 i)
-  LOCAL  (
-    lvar _sep (tarray tuchar 1) sep
+Definition update_rounds (non_empty_additional: bool): nat :=
+  if non_empty_additional then 2%nat else 1%nat.
+
+Definition update_loop_invariant_SEP (add_len: Z) (ctx additional K: val) (contents: list int) (key value: list Z) (final_state_abs: hmac256drbgabs) :mpred :=
+  EX state: _,
+  (data_at Tsh t_struct_hmac256drbg_context_st state ctx) *
+  (hmac256drbg_relate final_state_abs state) *
+  (data_at_ Tsh (tarray tuchar 32) K) *
+  (data_at Tsh (tarray tuchar add_len) (map Vint contents) additional).
+
+
+Definition update_loop_invariant (non_empty_additional: bool) (add_len: Z) (ctx additional sep K md_len: val) (contents: list int) (old_key old_value: list Z) (state_abs: hmac256drbgabs) (state: hmac256drbgstate) :=
+  EX i: _, EX key: _, EX value: _, EX final_state_abs: _,
+      PROP  (
+      (key, value) = HMAC_DRBG_update_round HMAC256 (map Int.signed contents) old_key old_value 0 i;
+      le i (update_rounds non_empty_additional);
+      key = hmac256drbgabs_key final_state_abs;
+      value = hmac256drbgabs_value final_state_abs;
+      hmac256drbgabs_metadata_same final_state_abs state_abs
+        )
+      LOCAL 
+      (temp _rounds
+         (force_val
+            (sem_cast_i2i I8 Unsigned
+               (if non_empty_additional
+                then Vint (Int.repr 2)
+                else Vint (Int.repr 1)))); temp _md_len md_len;
+      lvar _K (tarray tuchar 32) K; lvar _sep (tarray tuchar 1) sep;
+      temp _additional additional; temp _add_len (Vint (Int.repr add_len));
+      temp _sep_value (Vint (Int.repr (Z.of_nat i)))
          )
-  SEP  (
-  `(data_at Tsh (tarray tuchar 1) [Vint (Int.repr (Z.of_nat i))] sep);
-  `(data_at Tsh t_struct_hmac256drbg_context_st state ctx);
-  `(hmac256drbg_relate (hmac256drbgabs_update_key (hmac256drbgabs_update_value state_abs value) key) state)
-  ).
+      SEP  (
+        `(update_loop_invariant_SEP add_len ctx additional K contents key value final_state_abs)
+         ).
+
+Definition update_loop_pre_incr_invariant (non_empty_additional: bool) (add_len: Z) (ctx additional sep K md_len: val) (contents: list int) (old_key old_value: list Z) (state_abs: hmac256drbgabs) (state: hmac256drbgstate) :=
+  EX i: _, EX key: _, EX value: _, EX final_state_abs: _,
+      PROP  (
+      (key, value) = HMAC_DRBG_update_round HMAC256 (map Int.signed contents) old_key old_value 0 (i + 1);
+      lt i (update_rounds non_empty_additional);
+      key = hmac256drbgabs_key final_state_abs;
+      value = hmac256drbgabs_value final_state_abs;
+      hmac256drbgabs_metadata_same final_state_abs state_abs
+        )
+      LOCAL 
+      (temp _rounds
+         (force_val
+            (sem_cast_i2i I8 Unsigned
+               (if non_empty_additional
+                then Vint (Int.repr 2)
+                else Vint (Int.repr 1)))); temp _md_len md_len;
+      lvar _K (tarray tuchar 32) K; lvar _sep (tarray tuchar 1) sep;
+      temp _additional additional; temp _add_len (Vint (Int.repr add_len));
+      temp _sep_value (Vint (Int.repr (Z.of_nat i)))
+         )
+      SEP  (
+        `(update_loop_invariant_SEP add_len ctx additional K contents key value final_state_abs)
+         ).
+
+Definition update_loop_post (non_empty_additional: bool) (add_len: Z) (ctx additional sep K md_len: val) (contents: list int) (old_key old_value: list Z) (state_abs: hmac256drbgabs) (state: hmac256drbgstate) :=
+  EX key: _, EX value: _, EX final_state_abs:_,
+      PROP  (
+          (key, value) = HMAC_DRBG_update_round HMAC256 (map Int.signed contents) old_key old_value 0 (if non_empty_additional then 2%nat else 1%nat);
+          key = hmac256drbgabs_key final_state_abs;
+      value = hmac256drbgabs_value final_state_abs;
+      hmac256drbgabs_metadata_same final_state_abs state_abs
+        )
+      LOCAL 
+      (temp _rounds
+         (force_val
+            (sem_cast_i2i I8 Unsigned
+               (if non_empty_additional
+                then Vint (Int.repr 2)
+                else Vint (Int.repr 1)))); temp _md_len md_len;
+      lvar _K (tarray tuchar 32) K; lvar _sep (tarray tuchar 1) sep;
+      temp _additional additional; temp _add_len (Vint (Int.repr add_len))
+         )
+      SEP  (
+        `(update_loop_invariant_SEP add_len ctx additional K contents key value final_state_abs)
+         ).
+
 
 Lemma body_hmac_drbg_update: semax_body HmacDrbgVarSpecs HmacDrbgFunSpecs 
        f_mbedtls_hmac_drbg_update hmac_drbg_update_spec.
@@ -66,7 +134,7 @@ Proof.
       lvar _sep (tarray tuchar 1) sep;
       lvar _info (Tstruct _mbedtls_md_info_t noattr) info;
       temp _additional additional; temp _add_len (Vint (Int.repr add_len));
-      temp 126%positive (Val.of_bool non_empty_additional)
+      temp 127%positive (Val.of_bool non_empty_additional)
              )
       SEP  (`(data_at_ Tsh (tarray tuchar 32) K);
       `(data_at_ Tsh (tarray tuchar 1) sep);
@@ -84,12 +152,17 @@ Proof.
       {
         destruct additional'; try solve [inv TC].
         inversion TC. subst. solve_valid_pointer.
+        destruct contents.
+        (* contents = [], contradiction *)
+        assert (contra: False) by (apply H1; reflexivity); inversion contra.
+        (* contents != [], so pointer must be valid *)
+        entailer!.
+        rewrite Zlength_cons.
         admit (* TODO *).
       }
       solve_valid_pointer.
     }
     entailer!.
-    clear - H3 H1 TC.
     rewrite Zlength_map in *.
     destruct (eq_dec (Zlength contents) 0) as [zlength_eq | zlength_neq].
     assert (contra: False) by (apply H1; apply zlength_eq); inversion contra.
@@ -112,14 +185,14 @@ Proof.
     forward.
     entailer!.
   }
-
+  
   forward_if (
       PROP  ()
       LOCAL  (temp _md_len md_len; lvar _K (tarray tuchar 32) K;
       lvar _sep (tarray tuchar 1) sep;
       lvar _info (Tstruct _mbedtls_md_info_t noattr) info;
       temp _additional additional; temp _add_len (Vint (Int.repr add_len));
-      temp 127%positive (if non_empty_additional then (Vint (Int.repr 2)) else (Vint (Int.repr 1)))
+      temp 128%positive (if non_empty_additional then (Vint (Int.repr 2)) else (Vint (Int.repr 1)))
              )
       SEP  (`(data_at_ Tsh (tarray tuchar 32) K);
       `(data_at_ Tsh (tarray tuchar 1) sep);
@@ -140,8 +213,84 @@ Proof.
   }
   forward.
 
-  (* sep[0] = 0 *)
+  (* sep_value = 0 *)
+  unfold Sfor.
   forward.
 
-  forward.
+  (* for( ; sep_value < rounds; sep_value++ ) *)
+  remember (hmac256drbgabs_key initial_state_abs) as initial_key.
+  remember (hmac256drbgabs_value initial_state_abs) as initial_value.
+  forward_for
+    (update_loop_invariant non_empty_additional add_len ctx additional sep K md_len contents initial_key initial_value initial_state_abs initial_state)
+    (update_loop_pre_incr_invariant non_empty_additional add_len ctx additional sep K md_len contents initial_key initial_value initial_state_abs initial_state)
+    (update_loop_post non_empty_additional add_len ctx additional sep K md_len contents initial_key initial_value initial_state_abs initial_state).
+  {
+    (* show that pre-condition implies the invariant *)
+    unfold update_loop_invariant.
+    apply exp_right with 0%nat.
+    apply exp_right with initial_key.
+    apply exp_right with initial_value.
+    apply exp_right with initial_state_abs.
+    unfold update_loop_invariant_SEP.
+    entailer!.
+    destruct initial_state_abs; unfold hmac256drbgabs_metadata_same; auto.
+    apply exp_right with initial_state.
+    entailer!.
+    admit (* TODO *).
+  }
+  {
+    (* show that the loop check type-checks *)
+    entailer!.
+  }
+  {
+    (* prove the loop invariant + loop condition being false the post condition *)
+    remember (HMAC_DRBG_update_round HMAC256 (map Int.signed contents) initial_key initial_value 0 (if non_empty_additional then 2%nat else 1%nat)) as key_value_pair.
+    unfold update_loop_invariant.
+    unfold update_loop_post.
+    apply exp_right with (fst key_value_pair).
+    apply exp_right with (snd key_value_pair).
+    unfold update_loop_invariant_SEP.
+    unfold hmac256drbg_relate.
+    (*
+    entailer.
+    (* must intro the existential variables, then prove i = _rounds *)
+    entailer.
+    assert ((x >= update_rounds
+          (if eq_dec (Zlength (map Vint contents)) 0%Z
+           then false
+           else
+            if eq_dec (eval_id _additional rho) nullval then false else true))%nat). admit.
+    assert (x = update_rounds
+          (if eq_dec (Zlength (map Vint contents)) 0%Z
+           then false
+           else
+            if eq_dec (eval_id _additional rho) nullval then false else true)). admit.
+    subst. *)
+    admit (* TODO *).
+    (*
+    entailer.
+    {
+      repeat split.
+      {
+        symmetry; apply surjective_pairing.
+      }
+      {
+        destruct (eq_dec add_len 0).
+      }
+    }
+    {
+      entailer!.
+    }
+*)
+  }
+  {
+    (* prove the loop body + loop condition being true implies the loop pre-incr invariant *)
+    admit (* TODO *).
+  }
+  {
+    (* prove the pre-incr invariant preserves the invariant *)
+    unfold update_loop_pre_incr_invariant.
+    unfold update_loop_invariant_SEP.
+    admit (* TODO *).    
+  }
 Admitted.
